Weidenbach_Book/IsaSAT_LLVM.thy
@@ -377,7 +377,8 @@ sepref_def IsaSAT_code_wrapped
 
 experiment
 begin
-
+term NORMAL_PHASE
+declare NORMAL_PHASE_def[llvm_code]
   export_llvm IsaSAT_code_wrapped default_opts_impl IsaSAT_code file "code/isasat_restart.ll"
 
 end
