Weidenbach_Book/WB_More_IICF_LLVM.thy
@@ -1,7 +1,7 @@
 theory WB_More_IICF_LLVM
 imports 
   Isabelle_LLVM.IICF 
-  Isabelle_LLVM.Sepref_HOL_Bindings 
+  Isabelle_LLVM.Sepref_HOL_Bindings
   WB_More_Refinement
 begin
 
